@prefix : <http://msc.org/resources/MSC/msc2020/mscvocab#> .
@prefix owl: <http://www.w3.org/2002/07/owl#> .
@prefix rdf: <http://www.w3.org/1999/02/22-rdf-syntax-ns#> .
@prefix xml: <http://www.w3.org/XML/1998/namespace> .
@prefix xsd: <http://www.w3.org/2001/XMLSchema#> .
@prefix rdfs: <http://www.w3.org/2000/01/rdf-schema#> .
@base <http://msc.org/resources/MSC/msc2020/mscvocab> .
@prefix dc: <http://purl.org/dc/terms/> .
@prefix skos: <http://www.w3.org/2004/02/skos/core#> .

<http://msc.org/resources/MSC/msc2020/mscvocab> rdf:type owl:Ontology ;
                                                 owl:imports rdf: , skos: ;
                                                 rdfs:comment "This is an MSC-specific extension of SKOS created during the conversion of MSC 2020 to a SKOS vocabulary. It is based on <http://msc2010.org/resources/MSC/2010/mscvocab> created by Patrick Ion and Christoph Lange during their creation of a SKOS version of MSC 2010.";
                                                 dc:created "2021-03-15"^^xsd:date .

# Addition of properties to describe the ontology:

dc:creator a owl:AnnotationProperty .
dc:modified a owl:AnnotationProperty .
dc:created a owl:AnnotationProperty .

#################################################################
#    Object Properties
#################################################################

#Expanded after comparison with mscvocab-2010
###  http://msc.org/resources/MSC/msc2020/mscvocab#forTarget
:forTarget rdf:type owl:ObjectProperty ;
           rdfs:subPropertyOf rdf:object ;
           rdfs:label "target" ;
           rdfs:comment "target of a ‘see for’ link" ;
           rdfs:range skos:Concept ;
           rdfs:domain rdf:Statement; # maybe this is too general?
           skos:changeNote "In <http://msc2010.org/resources/MSC/2010/mscvocab> an instance of <http://msc2010.org/resources/MSC/2010/mscvocab#SeeForLink>, which is basically an instance of rdf:Statement was related to an instance of skos:Concept which was the object in a direct \"seeConditionally\" statement between two concepts. In MSC's 2020 SKOS version, we use rdf:object instead of this property."@en .

#Comment on related elements in this property from mscvocab-2010
<http://msc2010.org/resources/MSC/2010/mscvocab#SeeForLink> 
                rdfs:comment "Not taken over to mscvocab-2020. For reified links, with introduced classed that are subclasses of rdf:statement, e.g. :seeForStatement."@en ;
                skos:editorialNote "Mark this class as deprecated."@en ;
                rdfs:isDefinedBy <http://msc2010.org/resources/MSC/2010/mscvocab> .

# Expanded after comparison with mscvocab-2010
###  http://msc.org/resources/MSC/msc2020/mscvocab#relatedPartOf
:relatedPartOf rdf:type owl:ObjectProperty ;
        rdfs:label "partitively related" ;
        rdfs:subPropertyOf skos:semanticRelation .

# Expanded after comparison with mscvocab-2010
###  http://msc.org/resources/MSC/msc2020/mscvocab#seeAlso
:seeAlso rdf:type owl:ObjectProperty ;
        rdfs:label "see also" ;
         rdfs:subPropertyOf :relatedPartOf .

# Expanded after comparison with mscvocab-2010
###  http://msc.org/resources/MSC/msc2020/mscvocab#seeConditionally
:seeConditionally rdf:type owl:ObjectProperty ;
                  rdfs:label "see conditionally" ;
                  rdfs:subPropertyOf :relatedPartOf ;
                  owl:propertyChainAxiom (
   <http://msc2010.org/resources/MSC/2010/mscvocab#seeFor>
   rdf:object
 ) ;
 rdfs:comment "The owl:propertyChainAxiom defined in mscvocab-2010 has been updated to the new reification structure of MSC 2020 SKOS."@en .

#Expanded after comparison with mscvocab-2010
###  http://msc.org/resources/MSC/msc2020/mscvocab#seeFor
:seeFor rdf:type owl:ObjectProperty ;
        rdfs:label "for <some specific topic>, see" ;
        rdfs:comment "pointer to a record that describes a ‘see for’ link , i.e. an instance of mscvocab:seeForStatement"@en ;
        rdfs:range :seeForStatement ;
        rdfs:domain skos:Concept ;
        rdfs:subPropertyOf :relatedPartOf ;
        rdfs:comment "The rdfs:range defined in mscvocab-2010 of this property has been updated to the new reification structure of MSC 2020 SKOS."@en .

#Expanded after comparison with mscvocab-2010
###  http://msc.org/resources/MSC/msc2020/mscvocab#seeMainly
:seeMainly rdf:type owl:ObjectProperty ;
           rdfs:label "see mainly" ;
           rdfs:subPropertyOf :relatedPartOf .

#Updated IRI of inverse property
<http://msc2010.org/resources/MSC/2010/mscvocab#forSource>
  a owl:ObjectProperty ;
  rdfs:label "source" ;
  rdfs:comment "source of a ‘see for’ link" ;
  owl:inverseOf <http://msc.org/resources/MSC/msc2020/mscvocab#seeFor> ;
  rdfs:range skos:Concept .

#################################################################
#    Classes
#################################################################

###  http://msc.org/resources/MSC/msc2020/mscvocab#seeForStatement
:seeForStatement rdf:type owl:Class ;
                 rdfs:subClassOf rdf:Statement ;
                 rdfs:comment "Type of rdf:Statement that allows the annotation of a triple using mscvocab:seeConditionally/ reification of a triple using mscvocab:seeConcitionally. A :seeForStatement declares an rdf:subject, an rdf:predicate and an rdf:object and an mscvocab:scope that defines the condition of the reified triple using mscvocab:seeConditionally.";
                 skos:editorialNote "Newly introduced in mscvoca-2020, successor of <http://msc2010.org/resources/MSC/2010/mscvocab#SeeForLink>";
                 skos:editorialNote "Class IRI needs to be updated to follow CamelCase for classes. Update in MSC 2020 SKOS needed as well".

#Additions based on comparison between mscvocab-2010 and mscvocab-2020
<http://msc2010.org/resources/MSC/2010/mscvocab#MSCNotation>
  a rdfs:Datatype ;
  rdfs:label "MSC notation" ;
  owl:equivalentClass [
    a rdfs:Datatype ;
    owl:onDatatype <http://msc2010.org/resources/MSC/2010/mscvocab#string> ;
    owl:withRestrictions ( xsd:pattern "[0-9]{2}([A-Z-][0-9]{2}|-XX|[A-Z]xx)" )
  ] ;
  rdfs:comment "an MSC notation" .

<http://msc2010.org/resources/MSC/2010/mscvocab#string> a rdfs:Datatype .

#Taken over from mscvocab-2010 but not yet used by MSC 2020 SKOS, yet:
<http://msc2010.org/resources/MSC/2010/mscvocab#MustUseScopeNote>
  a owl:Class ;
  rdfs:label "‘must use’ scope note" ;
  rdfs:subClassOf <http://msc2010.org/resources/MSC/2010/mscvocab#ScopeNote> ;
  rdfs:comment "note on what additional classes must be used to classify a concept" .

<http://msc2010.org/resources/MSC/2010/mscvocab#NotUseScopeNote>
  a owl:Class ;
  rdfs:label "‘not use’ scope note" ;
  rdfs:subClassOf <http://msc2010.org/resources/MSC/2010/mscvocab#ScopeNote> ;
  rdfs:comment "note on what classes should not be used to classify a concept" .

<http://msc2010.org/resources/MSC/2010/mscvocab#ScopeNote>
  a owl:Class ;
  rdfs:label "scope note" ;
  rdfs:comment "note about the scope of a concept" .

<http://msc2010.org/resources/MSC/2010/mscvocab#UseScopeNote>
  a owl:Class ;
  rdfs:label "‘use’ scope note" ;
  rdfs:subClassOf <http://msc2010.org/resources/MSC/2010/mscvocab#ScopeNote> ;
  rdfs:comment "note on what additional classes should be used to classify a concept" .

[]
  a owl:AllDisjointClasses ;
  owl:members (
   <http://msc2010.org/resources/MSC/2010/mscvocab#MustUseScopeNote>
   <http://msc2010.org/resources/MSC/2010/mscvocab#NotUseScopeNote>
   <http://msc2010.org/resources/MSC/2010/mscvocab#UseScopeNote>
 ) .

<http://msc2010.org/resources/MSC/2010/mscvocab#scope>
  a owl:ObjectProperty ;
  rdfs:label "scope" ;
  rdfs:comment "used to restrict the scope of a link to a partitively related concept" ;
  rdfs:domain <http://msc2010.org/resources/MSC/2010/mscvocab#ScopeNote> ;
  rdfs:subPropertyOf skos:scopeNote .

<http://msc2010.org/resources/MSC/2010/mscvocab#matchDewey>
  a owl:ObjectProperty ;
  rdfs:label "matches Dewey Decimal Classification concept" ;
  rdfs:comment "link to a matching DDC concept (to be used until we know more exactly what kind of match it is, e.g. broad, exact, …)" ;
  rdfs:subPropertyOf skos:mappingRelation .

# New property to link an instance of skos:Concept to a skos:Collection
mscvocab:seeConditionallyElementofCollection a owl:ObjectProperty ;
  rdfs:label "Property used to link an MSC concept to a collection of other MSC concepts when a certain condition is met";
  rdfs:domain skos:Collection .
###  Generated by the OWL API (version 4.5.9.2019-02-01T07:24:44Z) https://github.com/owlcs/owlapi
