Prefix: : <http://msc2010.org/resources/MSC/2010/mscvocab#>

Prefix: skos:    <http://www.w3.org/2004/02/skos/core#>
Prefix: dcterms: <http://purl.org/dc/terms/>

AnnotationProperty: dcterms:created
AnnotationProperty: dcterms:creator
AnnotationProperty: dcterms:modified

Ontology: <http://msc2010.org/resources/MSC/2010/mscvocab>
  Annotations: rdfs:comment "MSC-specific extension of the SKOS vocabulary.  This ontology is actually intended to import and extend SKOS Core, but as that doesn't work with Protégé, we redeclare part of SKOS here.  So far, the primary reference for the design considerations underlying this ontology is the following the following publication:\nChristoph Lange, Patrick Ion, Anastasia Dimou, Charalampos Bratsas, Wolfram Sperber, Michael Kohlhase, and Ioannis Antoniou: Getting Mathematics Towards the Web of Data: the Case of the Mathematics Subject Classification.  In: Elena Paslaru Bontas Simperl et al. (eds.), 9th Extended Semantic Web Conference (ESWC).  Hersonissos, Crete, Greece.  Lecture Notes in Computer Science, Springer, 2012.",
    rdfs:label "Mathematics Subject Classification (MSC2010)",
    dcterms:creator "Christoph Lange",
    dcterms:creator "Patrick Ion",
    dcterms:modified "2012-03-10"^^xsd:date,
    dcterms:created "2012-02-16"^^xsd:date
  # Import: skos:

# Protégé does not support importing the actual SKOS ontology, so we just redeclare the relevant SKOS vocabulary:
ObjectProperty: skos:semanticRelation
ObjectProperty: skos:mappingRelation
ObjectProperty: skos:changeNote
ObjectProperty: skos:scopeNote
Class: skos:Concept

# Our actual vocabulary starts here:
ObjectProperty: relatedPartOf
  Annotations: rdfs:label "partitively related"
  SubPropertyOf: skos:semanticRelation

# TODO maybe comment on symmetry vs. non-symmetry of this property (cf. http://trac.mathweb.org/msc/ticket/9)
ObjectProperty: seeAlso
  Annotations: rdfs:label "see also"
  SubPropertyOf: relatedPartOf

# FIXME some "seeMainly" links in the SKOS are broken, as they contain additional text.  Figure out how to handle this.
ObjectProperty: seeMainly
  Annotations: rdfs:label "see mainly"
  SubPropertyOf: relatedPartOf

ObjectProperty: seeConditionally
  Annotations: rdfs:label "see conditionally"
  SubPropertyOf: relatedPartOf
  SubPropertyChain: seeFor o forTarget

ObjectProperty: seeFor
  Annotations: rdfs:comment "pointer to a record that describes a ‘see for’ link",
    rdfs:label "for <some specific topic>, see"
  Domain: skos:Concept
  Range: SeeForLink

ObjectProperty: forSource
  Annotations: rdfs:label "source",
    rdfs:comment "source of a ‘see for’ link"
  Range: skos:Concept
  InverseOf: seeFor

ObjectProperty: forTarget
  Annotations: rdfs:label "target",
    rdfs:comment "target of a ‘see for’ link"
  Domain: SeeForLink
  Range: skos:Concept

ObjectProperty: formerlyNote
  Annotations: rdfs:label "note (formerly)",
    # FIXME clarify; see http://trac.mathweb.org/msc/ticket/7
    owl:deprecated "true"^^xsd:boolean
  SubPropertyOf: skos:changeNote
  Range: FormerlyNote

# FIXME currently also used to express that some concepts are just placeholders for DDC concepts (see https://trac.mathweb.org/msc/ticket/50)
ObjectProperty: scope
  Annotations: rdfs:label "scope",
    rdfs:comment "used to restrict the scope of a link to a partitively related concept"
  SubPropertyOf: skos:scopeNote
  Domain: ScopeNote

ObjectProperty: matchDewey
  Annotations: rdfs:label "matches Dewey Decimal Classification concept",
    rdfs:comment "link to a matching DDC concept (to be used until we know more exactly what kind of match it is, e.g. broad, exact, …)"
  SubPropertyOf: skos:mappingRelation

Class: FormerlyNote
  Annotations: rdfs:label "‘Formerly’ note",
    rdfs:comment "note about former use of a concept"

Class: ScopeNote
  Annotations: rdfs:label "scope note",
    rdfs:comment "note about the scope of a concept"

Class: UseScopeNote
  Annotations: rdfs:label "‘use’ scope note",
    rdfs:comment "note on what additional classes should be used to classify a concept"
  SubClassOf: ScopeNote
  
Class: NotUseScopeNote
  Annotations: rdfs:label "‘not use’ scope note",
    rdfs:comment "note on what classes should not be used to classify a concept"
  SubClassOf: ScopeNote

Class: MustUseScopeNote
  Annotations: rdfs:label "‘must use’ scope note",
    rdfs:comment "note on what additional classes must be used to classify a concept"
  SubClassOf: ScopeNote

DisjointClasses: UseScopeNote, NotUseScopeNote, MustUseScopeNote

Class: SemanticRelation
  Annotations: rdfs:label "semantic relation",
    rdfs:comment "superclass of all MSC-specific types of reified links"

Class: SeeForLink
  Annotations: rdfs:label "‘see for’ link",
    rdfs:comment "reified link from one concept to a partitively related concept"
  SubClassOf: SemanticRelation

Datatype: MSCNotation
  Annotations: rdfs:label "MSC notation",
    rdfs:comment "an MSC notation"
  EquivalentTo: string[pattern "[0-9]{2}([A-Z-][0-9]{2}|-XX|[A-Z]xx)"]

